reverse path diretion

bfs.v
@@ -133,77 +133,47 @@ Lemma no_aliens : forall g s parent, bfs g s = parent ->
     exists neighbors, In (v, neighbors) g /\ In u neighbors.
 Abort.
 
+Definition path := (node * list node)%type.
+Definition destination (p:path) := fst p.
+Definition route (p:path) := snd p.
+Definition length (p : path) : nat := length (route p).
+Definition startNode (p : path) : node := last (route p) (destination p).
+
 (* This assumes that the statement (u's parent is v) comes before any statement
  about v's parents. This is true in out BFS implementation, and will probably
  remain true for any extension of it, but it is not an integral property of BFS
  -- it is just a requirement on the output format. We could get rid of this
  requirement, but then the termination argument for traceParent would depend on
- the assumption that parsing the parent map does not lead to cyclic paths. *)
-Fixpoint traceParent (parent:parent_t) (u:node) {struct parent} : list node :=
+ the assumption that parsing the parent map does not lead to cyclic paths.  We
+ plan to prove things about the output of traceParent when it is run on the
+ output of bfs, so thedivision of labor between the two should not matter a
+ whole lot. *)
+Fixpoint traceParent' (parent:parent_t) (u:node) {struct parent} : list node :=
   match parent with
   | nil => []
   | p::parent' =>
     if node_eq_dec (fst p) u
-    then (snd p)::(traceParent parent' (snd p))
-    else traceParent parent' u
+    then (snd p)::(traceParent' parent' (snd p))
+    else traceParent' parent' u
 end.
-
-Lemma bfs_paths_start : forall g s parent, bfs g s = parent ->
-   forall v p, traceParent parent v = p -> p <> nil ->
-   forall d, In (last p d) s.
-Abort.
+Definition traceParent (parent:parent_t) (u:node) := (u, traceParent' parent u).
 
 Example ex2 :
-  traceParent [(Node 3, Node 2); (Node 2, Node 0); (Node 1, Node 0)] (Node 3) =
+  traceParent' [(Node 3, Node 2); (Node 2, Node 0); (Node 1, Node 0)] (Node 3) =
   [Node 2; Node 0].
 Abort. (* Why does this not work again... *)
-
-Inductive path : Type :=
-  | Starts : node -> path
-  | Cons : path -> node -> path.
 
 Definition hasEdge (g : graph) (n1 n2 : node) : Prop :=
   exists (neighbors : list node), In (n1, neighbors) g /\ In n2 neighbors.
 
-Fixpoint length (p : path) : nat :=
-  match p with
-    | Starts _ => 0
-    | Cons p' _ => S(length p')
-  end.
-
-Fixpoint startNode (p : path) : node :=
-  match p with
-    | Starts n => n
-    | Cons p' _ => startNode p'
-  end.
-
-Definition endNode (p : path) : node :=
-  match p with
-    | Starts n => n
-    | Cons _ n => n
-  end.
-
 Definition nodes (g : graph) := edgeStarts g. (* TODO: dummy *)
 
-(* Fixpoint hasPath (g : graph) (p : path) : Prop :=
-     match p with
-       | Starts n => In n (nodes g)
-       | Cons p' n => match p' with
-                        | Starts n' => hasEdge g n' n
-                        | Cons _ n' => hasEdge g n' n /\ hasPath g p'
-                      end
-     end.*)
-
 Inductive hasPath : graph -> path -> Prop :=
-| IdPath : forall g n, In n (nodes g) -> hasPath g (Starts n)
-| ConsPath : forall g n n' p', hasPath g p' ->
-             endNode p' = n -> hasEdge g n n' -> hasPath g (Cons p' n').
+| IdPath : forall g n, In n (nodes g) -> hasPath g (n, [])
+| ConsPath : forall g n n' r', hasEdge g n n' -> hasPath g (n, r') -> hasPath g (n', n::r').
 
 Definition reachable (startn : node) (endn : node) (g : graph) : Prop :=
-  exists (p : path), hasPath g p /\ startNode p = startn /\ endNode p = endn.
-
-Definition paths_from_parents (p:parent_t) : list path :=
-  nil. (* TODO: put the real def in *)
+  exists (p : path), hasPath g p /\ startNode p = startn /\ destination p = endn.
 
 (* Tõestada: kui paths_from_parents väljastab pathi, siis path_in_graph.
    Tõestada: kui paths_from_parents väljastab pathi, siis In frontier (startNode p) *)
@@ -228,9 +198,9 @@ Definition bfs_finds_shortest : Prop :=
   forall (g : graph) (frontier : list node) (n1 : node) (n2 : node),
     In n1 frontier -> reachable n1 n2 g ->
     exists (p : path), In p (paths_from_parents (bfs g frontier)) /\
-      n1 = startNode p /\ n2 = endNode p /\
+      n1 = startNode p /\ n2 = destination p /\
       (forall (p' : path), n1 = startNode p' ->
-         n2 = endNode p' -> hasPath g p' ->
+         n2 = destination p' -> hasPath g p' ->
          length p' >= length p).
 
 (* Tõestada: kõik, mis BFS leiab, on lühimad *)
